bce/bce_proof.dfy
@@ -126,17 +126,131 @@ lemma lemma_BCE_Validity_Correct_Nodes_Decide_Codeword(s':Service, syndromes: se
         var syndromes_received := syndromes[node.id];  // seq of syndromes received by node.id
         assert syndromes_received == extractSyndromes(s'.nodes);
         lemma_Extracted_Syndromes_Are_Computed(s'.nodes);
+
+        // Prove that my own computed syndrome is good
         var my_syndrome := syndromes_received[node.id]; // syndome computed by node.id for itself
         assert node == s'.nodes[node.id];
         assert my_syndrome == computeSyndrome(node);
         lemma_Computed_Syndromes_Have_Length_n(node, my_syndrome);
         lemma_BCE_Validity_Correct_Nodes_Own_Syndrome_Is_Good(node, my_syndrome);
-        assert countTrue(syndromes_received[node.id]) >= node.n - node.f;
-        assert countGoodSyndromes(syndromes_received, node.n-node.f) >= node.n - node.f;
+        assert countTrue(my_syndrome) >= node.n - node.f;
+
+        // Prove that n-f of received syndromes are good
+        assert forall i :: 0 <= i < s'.n ==> syndromes_received[i] == computeSyndrome(s'.nodes[i]);
+        lemma_BCE_Validity_CountGoodSyndromes_Succeeds(s', node, syndromes_received);
     }
 }
 
 
+/* Prove that for any non-faulty node n, countTrue(computeSyndrome(n)) >= n - f */
+// TODO
+lemma lemma_BCE_Validity_Correct_Nodes_Send_Good_Syndrome(s':Service, node: Node, syndromes_received: seq<syndrome>) 
+    requires node_invariants(s');
+    requires |s'.nodes| == s'.n;
+    requires forall  i :: 0 <= i < s'.n ==> s'.nodes[i].id == i
+    requires node in s'.nodes;
+    requires forall n :: n in s'.nodes ==> n.n == |n.symbols| == |n.codeword|;
+    // requires forall node :: 
+    //     node in s'.nodes && !node.faulty
+    //     ==>
+    //     && node.symbols == node.codeword  //by "everyone is behaving" temporary assumption
+    //     && node.state == Phase2
+    //     && 0 <= node.id < s'.n
+    requires |syndromesToExchange(s'.nodes)| == s'.n;
+    requires syndromes_received == syndromesToExchange(s'.nodes)[node.id];
+    requires |syndromes_received| == s'.n;
+    requires forall i :: 0 <= i < s'.n ==> syndromes_received[i] == computeSyndrome(s'.nodes[i]);
+    ensures forall id :: 0 <= id < s'.n 
+        ==> 
+        (!s'.nodes[id].faulty ==> countTrue(computeSyndrome(s'.nodes[id])) >= node.n - node.f);
+{}
+
+
+// TODO
+lemma {:induction syndromes_received} lemma_BCE_Validity_CountGoodSyndromes_Succeeds(s':Service, node: Node, syndromes_received: seq<syndrome>) 
+    requires node_invariants(s');
+    requires |s'.nodes| == s'.n;
+    requires forall  i :: 0 <= i < s'.n ==> s'.nodes[i].id == i
+    requires node in s'.nodes;
+    requires forall n :: n in s'.nodes ==> n.n == |n.symbols| == |n.codeword|;
+    // requires forall node :: 
+    //     node in s'.nodes && !node.faulty
+    //     ==>
+    //     && node.symbols == node.codeword  //by "everyone is behaving" temporary assumption
+    //     && node.state == Phase2
+    //     && 0 <= node.id < s'.n
+    requires |syndromesToExchange(s'.nodes)| == s'.n;
+    requires syndromes_received == syndromesToExchange(s'.nodes)[node.id];
+    requires |syndromes_received| == s'.n;
+    requires forall i :: 0 <= i < s'.n ==> syndromes_received[i] == computeSyndrome(s'.nodes[i]);
+    ensures countGoodSyndromes(syndromes_received, node.n-node.f) >= s'.n - s'.f;
+{
+    lemma_BCE_Validity_Correct_Nodes_Send_Good_Syndrome(s', node, syndromes_received);
+    lemma_BCE_Validity_CountGoodSyndromes_Succeeds_Helper(s', node, syndromes_received, s'.n, s'.f);
+}
+
+
+// TODO
+lemma {:induction i, f} lemma_BCE_Validity_CountGoodSyndromes_Succeeds_Helper(s':Service, node: Node, syndromes_received: seq<syndrome>, i: int, f: int) 
+    decreases i, f;
+    requires node_invariants(s');
+    requires 0 <= i <= s'.n;
+    requires 0 <= f <= s'.f;
+    requires |s'.nodes| == s'.n;
+    requires forall  id :: 0 <= id < s'.n ==> s'.nodes[id].id == id
+    requires node in s'.nodes;
+    requires forall n :: n in s'.nodes ==> n.n == |n.symbols| == |n.codeword|;
+    requires |syndromesToExchange(s'.nodes)| == s'.n;
+    requires syndromes_received == syndromesToExchange(s'.nodes)[node.id];
+    requires |syndromes_received| == s'.n;
+    requires forall id :: 0 <= id < s'.n ==> syndromes_received[id] == computeSyndrome(s'.nodes[id]);
+    requires forall id :: 0 <= id < s'.n ==> 
+        (!s'.nodes[id].faulty ==> countTrue(computeSyndrome(s'.nodes[id])) >= s'.n - s'.f)
+    ensures countGoodSyndromes(syndromes_received[..i], node.n-node.f) >= i - f;
+{
+    var thresh := s'.n - s'.f;
+    if i == 0 {
+        assert countGoodSyndromes(syndromes_received[..i], thresh) == 0;
+    } else {
+        // Check the next syndrome (ith) for goodness
+        if !s'.nodes[i-1].faulty {
+            lemma_BCE_Validity_CountGoodSyndromes_Succeeds_Helper(s', node, syndromes_received, i-1, f);
+            var check_prefix := syndromes_received[..i];
+            var x := countTrue(check_prefix[|check_prefix|-1]);
+            assert x >= thresh;
+            assert countGoodSyndromes(check_prefix, thresh) ==
+                1 + countGoodSyndromes(check_prefix[..|check_prefix|-1], thresh);
+            assert check_prefix[..|check_prefix|-1] == syndromes_received[..i-1];
+        } else {
+            if f > 0 {
+                lemma_BCE_Validity_CountGoodSyndromes_Succeeds_Helper(s', node, syndromes_received, i-1, f-1);
+                var check_prefix := syndromes_received[..i];
+                var x := countTrue(check_prefix[|check_prefix|-1]);
+                if x >= thresh {
+                    assert countGoodSyndromes(check_prefix, thresh) ==
+                        1 + countGoodSyndromes(check_prefix[..|check_prefix|-1], thresh);
+                    assert check_prefix[..|check_prefix|-1] == syndromes_received[..i-1];
+                } else {
+                    assert countGoodSyndromes(check_prefix, thresh) == countGoodSyndromes(check_prefix[..|check_prefix|-1], thresh);
+                    assert check_prefix[..|check_prefix|-1] == syndromes_received[..i-1];
+                }
+            } else {
+                // Every node seen must be correct from this point
+                lemma_BCE_Validity_CountGoodSyndromes_Succeeds_Helper(s', node, syndromes_received, i-1, f);
+                var check_prefix := syndromes_received[..i];
+                assert !s'.nodes[i-1].faulty;
+                var x := countTrue(check_prefix[|check_prefix|-1]);
+                assert x >= thresh;
+                assert countGoodSyndromes(check_prefix, thresh) ==
+                    1 + countGoodSyndromes(check_prefix[..|check_prefix|-1], thresh);
+                assert check_prefix[..|check_prefix|-1] == syndromes_received[..i-1];
+            }
+        }
+    }
+}
+
+
+/* Prove that for any correct node, its own syndrome has n-f 'true' bits */
 lemma {:induction my_syndrome} lemma_BCE_Validity_Correct_Nodes_Own_Syndrome_Is_Good(node: Node, my_syndrome: syndrome) 
     requires !node.faulty;
     requires node.state == Phase2;
@@ -148,7 +262,7 @@ lemma {:induction my_syndrome} lemma_BCE_Validity_Correct_Nodes_Own_Syndrome_Is_
     ensures countTrue(my_syndrome) >= node.n - node.f;
 {
     assert |computeSyndrome(node)| == node.n;
-    assert my_syndrome[0..node.n] == my_syndrome;
+    assert my_syndrome[..node.n] == my_syndrome;
     lemma_BCE_Validity_Correct_Nodes_Own_Syndrome_Is_Good_Helper(node, my_syndrome, node.n);
 }
 
@@ -163,22 +277,22 @@ lemma {:induction i} lemma_BCE_Validity_Correct_Nodes_Own_Syndrome_Is_Good_Helpe
     requires node.symbols == node.codeword; //by "everyone is behaving" temporary assumption
     requires my_syndrome == computeSyndrome(node);
     requires 0 <= i <= node.n;
-    ensures countTrue(my_syndrome[0..i]) >= i - node.f;
+    ensures countTrue(my_syndrome[..i]) >= i - node.f;
 {
     if i == 0 {
-        assert my_syndrome[0..i] == [];
-        assert countTrue(my_syndrome[0..i]) == 0;
+        assert my_syndrome[..i] == [];
+        assert countTrue(my_syndrome[..i]) == 0;
     } else {
         lemma_BCE_Validity_Correct_Nodes_Own_Syndrome_Is_Good_Helper(node, my_syndrome, i-1);
-        assert countTrue(my_syndrome[0..i-1]) >= i-1 - node.f;
+        assert countTrue(my_syndrome[..i-1]) >= i-1 - node.f;
         assert node.symbols[i-1] == node.codeword[i-1];
         lemma_Computed_Syndromes_Is_Correct(node, my_syndrome);
         assert my_syndrome[i-1] == true;
-        var prefix := my_syndrome[0..i];
+        var prefix := my_syndrome[..i];
         assert |prefix| > 0;
         assert prefix[|prefix|-1] == true;
-        assert countTrue(prefix) == 1 + countTrue(prefix[0..|prefix|-1]);
-        assert my_syndrome[0..i-1] == prefix[0..|prefix|-1];
+        assert countTrue(prefix) == 1 + countTrue(prefix[..|prefix|-1]);
+        assert my_syndrome[..i-1] == prefix[..|prefix|-1];
     }
 }
 }
